src/ParametricInline.v
@@ -1,4 +1,172 @@
-Require Import PartialInline ParametricSyntax ParametricEquiv Syntax String List Semantics.
+Require Import PartialInline
+        PartialInline2 ParametricSyntax ParametricEquiv Syntax String List Semantics
+        Lib.Struct Program.Equality Lib.CommonTactics.
+
+Section concat_app.
+  Variable A: Type.
+  Lemma concat_app: forall l1 l2: list (list A), concat (l1 ++ l2) = concat l1 ++ concat l2.
+  Proof.
+    induction l1; simpl in *; auto; intros.
+    rewrite <- app_assoc.
+    f_equal; auto.
+  Qed.
+End concat_app.
+
+Section NoDup.
+  Variable A: Type.
+  Lemma noDupApp l1: forall l2, NoDup l1 -> NoDup l2 ->
+                                (forall i: A, In i l1 -> ~ In i l2) ->
+                                NoDup (l1 ++ l2).
+  Proof.
+    induction l1; simpl in *; intros.
+    - intuition.
+    - inv H.
+      specialize (IHl1 _ H5 H0).
+      assert (forall i, In i l1 -> ~ In i l2) by (intros; apply H1; intuition).
+      specialize (IHl1 H).
+      assert (~ In a l2) by (intros; apply H1; auto).
+      constructor; auto.
+      unfold not; intros K; apply in_app_or in K.
+      destruct K; intuition auto.
+  Qed.
+End NoDup.
+
+Section AboutConcat.
+  Variable A: Type.
+
+  Lemma in_concat_iff (ls: list (list A)):
+    forall x,
+      In x (concat ls) -> exists l, In l ls /\ In x l.
+  Proof.
+    induction ls; simpl in *; auto; intros; intuition auto.
+    apply in_app_or in H.
+    destruct H.
+    exists a; intuition auto.
+    specialize (IHls _ H); dest.
+    exists x0; auto.
+  Qed.
+
+  Lemma in_concat_iff2 (ls: list (list A)):
+    forall x,
+      In x (concat ls) -> exists i, In x (nth i ls nil).
+  Proof.
+    induction ls; simpl in *; auto; intros; intuition auto.
+    apply in_app_or in H.
+    destruct H.
+    exists 0; intuition auto.
+    specialize (IHls _ H); dest.
+    exists (S x0); auto.
+  Qed.
+
+
+  Variable B: Type.
+  Variable f: A -> B.
+  Lemma map_concat: forall (l: list (list A)) x, In x (map f (concat l)) ->
+                                                 In x (concat (map (map f) l)).
+  Proof.
+    induction l; simpl in *; auto; intros.
+    rewrite map_app in *.
+    apply in_app_or in H.
+    apply in_or_app.
+    destruct H; auto.
+  Qed.
+End AboutConcat.
+
+Section NoDup2.
+  Variable l: list MetaMeth.
+  Lemma noDup_preserve: NoDup (map getMetaMethName l) ->
+                        NoDup (namesOf (concat (map getListFromMetaMeth l))).
+  Proof.
+    induction l; simpl in *; auto; intros.
+    dependent destruction H.
+    specialize (IHl0 H0).
+    unfold namesOf; rewrite map_app;
+    fold (namesOf (getListFromMetaMeth a));
+    fold (namesOf (concat (map getListFromMetaMeth l0))).
+    apply noDupApp; auto; unfold not; intros.
+    - destruct a; simpl in *; auto.
+      unfold repMeth, getListFromRep, namesOf; simpl.
+      rewrite map_map; simpl.
+      clear - goodStrFn2 ls noDup.
+      induction ls; simpl; intros; [auto|].
+      inv noDup; constructor; auto.
+      unfold not; intros.
+      apply in_map_iff in H; dest.
+      specialize (goodStrFn2 _ _ _ _ H); dest; subst.
+      auto.
+    - destruct a; simpl in *; auto.
+      destruct H1; auto; subst.
+      unfold namesOf in H2; apply in_map_iff in H2; dest; subst.
+
+      destruct x.
+      destruct attrType; simpl in *.
+      apply in_concat_iff in H2; dest.
+      apply in_map_iff in H2; dest; subst.
+      unfold getListFromMetaMeth in H3; simpl in H3.
+
+      
+      destruct x1; simpl in *; auto.
+      inv H3; subst; auto.
+      destruct s0, s; simpl in *.
+      inv H1.
+      destruct_existT.
+      assert (In nameVal0 (map getMetaMethName l0)).
+      { apply in_map_iff.
+        exists (OneMeth b0 {| nameVal := nameVal0; goodName := goodName |}); simpl; auto.
+      }
+      intuition auto.
+
+      
+      unfold repMeth, getListFromRep in H3.
+      apply in_map_iff in H3; dest.
+      inv H1; destruct_existT.
+      destruct s0, s; simpl in *.
+      rewrite <- H5 in *.
+      unfold addIndexToStr in goodName0.
+      apply (badIndex _ _ goodName0).
+
+      
+      unfold repMeth, getListFromRep in H1.
+      unfold namesOf in H1, H2.
+      
+      apply in_map_iff in H1.
+      apply in_map_iff in H2.
+      dest; subst.
+      destruct x0, x.
+      destruct attrType, attrType0.
+      simpl in *.
+      apply in_map_iff in H4; dest.
+      apply in_concat_iff in H3; dest.
+      apply in_map_iff in H3; dest; subst.
+      unfold getListFromMetaMeth in H5.
+      inv H1; destruct_existT; subst.
+      destruct x3; simpl in *.
+      destruct H5; [|auto].
+      inv H1; destruct_existT; subst.
+      destruct s0; simpl in *; subst.
+      unfold addIndexToStr in goodName.
+      apply (badIndex _ _ goodName).
+      unfold repMeth, getListFromRep in H5.
+      apply in_map_iff in H5; dest; subst.
+      inv H1; destruct_existT; subst.
+      unfold addIndexToStr in H5.
+      assert (nameVal s <> nameVal s0).
+      { unfold not; intros.
+        rewrite H1 in H.
+        apply in_map with (f := getMetaMethName) in H6; simpl in H6.
+        auto.
+      }
+      clear - H5 H1.
+      destruct s, s0; simpl in *.
+      match goal with
+        | H: ?s1 = ?s2 |- _ => assert (substring 0 (String.length nameVal0) s1 =
+                                       substring 0 (String.length nameVal0) s2)
+                                      by (f_equal; auto)
+      end.
+                                                                      
+    
+  Qed.
+End NoDup2.
 
 Section GenGen.
   Variable m: MetaModule.
@@ -7,33 +175,65 @@ Section GenGen.
   Variable A: Type.
   Variable strA: A -> string.
   Variable goodStrFn: forall i j, strA i = strA j -> i = j.
+  Variable GenK: Kind.
+  Variable getConstK: A -> ConstT GenK.
   Variable goodStrFn2: forall si sj i j, addIndexToStr strA i si = addIndexToStr strA j sj ->
                                          si = sj /\ i = j.
-  Variable dm: sigT GenMethodT.
+  Variable dm: sigT (GenMethodT GenK).
   Variable dmName: string.
+  Variable preDm sufDm: list MetaMeth.
   Variable ls: list A.
+  Variable noDupLs: NoDup ls.
+  Variable Hdm: metaMeths m =
+                preDm ++ RepMeth strA goodStrFn getConstK goodStrFn2 dm dmName ls :: sufDm.
 
-  Variable r: GenAction Void.
+  Variable r: GenAction GenK Void.
   Variable rName: string.
+  Variable preR sufR: list MetaRule.
+  Variable Hrule: metaRules m =
+                  preR ++ RepRule strA goodStrFn getConstK goodStrFn2 r rName ls :: sufR.
 
-  Hypotheses (Hdm: In (RepMeth strA goodStrFn goodStrFn2 dm dmName ls) (metaMeths m))
-             (HnoDupMeths: NoDup (map getMetaMethName (metaMeths m)))
+  Hypotheses (HnoDupMeths: NoDup (map getMetaMethName (metaMeths m)))
              (HnoDupRules: NoDup (map getMetaRuleName (metaRules m))).
-  Hypothesis Hrule: In (RepRule strA goodStrFn goodStrFn2 r rName ls) (metaRules m).
 
-  Lemma InlineGenGenDmToRule_traceRefines_1:
+  Lemma InlineGenGenDmToRule_traceRefines_NoFilt:
     makeModule m <<==
                makeModule
                {| metaRegs := metaRegs m;
                   metaRules :=
-                    map (fun newr =>
-                           if string_dec rName (getMetaRuleName newr)
-                           then RepRule strA goodStrFn goodStrFn2
-                                        (fun ty => inlineGenGenDm (r ty) dmName dm) rName ls
-                           else newr) (metaRules m);
+                    preR ++ RepRule strA goodStrFn getConstK goodStrFn2
+                         (fun ty => inlineGenGenDm (r ty) dmName dm) rName ls :: sufR;
                   metaMeths := metaMeths m |}.
   Proof.
-    admit.
+    unfold makeModule; simpl.
+    rewrite Hrule.
+    repeat rewrite map_app; simpl.
+    repeat rewrite concat_app; simpl.
+    unfold repRule at 2; unfold getListFromRep.
+    rewrite mapFoldInlineDmsGenGen_matchesGen; auto.
+    rewrite Hdm.
+    repeat rewrite map_app; simpl.
+    repeat rewrite concat_app; simpl.
+    match goal with
+      | H: metaMeths m = ?l |- _ =>
+        assert (sth1: concat (map getListFromMetaMeth (metaMeths m)) =
+                concat (map getListFromMetaMeth l))
+          by (rewrite H; reflexivity);
+          repeat rewrite map_app in sth1; simpl in sth1; repeat rewrite concat_app in sth1;
+          simpl in sth1
+    end.
+    match goal with
+      | H: metaRules m = ?l |- _ =>
+        assert (sth2: concat (map getListFromMetaRule (metaRules m)) =
+                concat (map getListFromMetaRule l))
+          by (rewrite H; reflexivity);
+          repeat rewrite map_app in sth2; simpl in sth2; repeat rewrite concat_app in sth2;
+          simpl in sth2
+    end.
+    apply inlineDmsToRules_traceRefines_NoFilt
+    with (preDm := concat (map getListFromMetaMeth preDm))
+           (sufDm := concat (map getListFromMetaMeth sufDm)); auto; simpl;
+    [rewrite <- sth1 | rewrite <- sth2].
   Qed.
 
   Hypothesis HnoRuleCalls: forall rule,
